src/Assembly/State.v
@@ -175,7 +175,7 @@ Module Triple_as_OT <: UsualOrderedType.
 End Triple_as_OT.
 
 Module StateCommon.
-  Export ListNotations Util.
+  Export ListNotations.
 
   Module NatM := FMapAVL.Make(Nat_as_OT).
   Module PairM := FMapAVL.Make(Pair_as_OT).
